examples/modfair/ModFairAproof.v
@@ -1,0 +1,179 @@
+Require Import ModFairA.
+Require Import HoareDef SimModSem.
+Require Import Coqlib.
+Require Import ImpPrelude.
+Require Import Skeleton.
+Require Import PCM.
+Require Import ModSem ModSemE Behavior.
+Require Import Relation_Definitions.
+
+(*** TODO: export these in Coqlib or Universe ***)
+Require Import Relation_Operators.
+Require Import RelationPairs.
+From ITree Require Import
+     Events.MapDefault.
+From ExtLib Require Import
+     Core.RelDec
+     Structures.Maps
+     Data.Map.FMapAList.
+Require Import HTactics ProofMode IPM.
+Require Import OpenDef.
+Require Import Mem1 STB Invariant.
+
+Require Import IProofMode IRed ITactics.
+
+Require Import sProp sWorld World SRF.
+From stdpp Require Import coPset gmap namespaces.
+
+Require Import WFLibLarge FairCounter.
+
+Set Implicit Arguments.
+
+Local Open Scope nat_scope.
+
+Section SIMMODSEM.
+  Context `{_W: CtxWD.t}.
+
+  Variable id: ID.
+        
+  Variable GlobalStb: Sk.t -> gname -> option fspec.
+  Hypothesis STBINCLM: forall sk, stb_incl (to_stb (FairStb id)) (GlobalStb sk).
+
+  (* IST when iimap of the src and tgt change at the same time *)
+
+  Definition middle_update isrc itgt f: iimap id owf := 
+    (fun x => match f x with
+              | Flag.success => Ord.omega
+              | Flag.fail => Ord.from_nat (itgt x)
+              | _ => isrc x 
+              end).
+
+  Definition IstFair: Any.t -> Any.t -> iProp :=
+    fun st_src st_tgt => 
+      (⌜exists (itgt: iimap id nat_wf) (isrc: iimap id owf), 
+        st_tgt = itgt↑ ∧ st_src = isrc↑
+        ∧ forall f, fair_update id owf isrc (middle_update isrc itgt f) f⌝)%I.
+
+  Definition i_omega: iimap id owf := fun x => Ord.omega.
+
+  Lemma simF_fair:
+    forall (i_tgt: iimap id nat_wf),
+    HModPair.sim_fun
+      (ModFairA.HFair i_omega)
+      (ModFairA.HFair i_tgt)
+      IstFair "fair".
+  Proof.
+    simF_init HFair_unfold HFair_unfold fairF fairF.
+    st. iDestruct "ASM" as "[W [% %]]"; des; subst.
+    
+    rewrite Any.upcast_downcast in G. inv G. ss. inv G0.
+
+    force_r. instantiate (1:=mk_meta y0 y1 ()). force_r. force_r. iSplitR "IST".
+    { iFrame; et. }
+    st. iDestruct "IST" as "%"; des; subst.
+    
+    rewrite Any.upcast_downcast in G1. symmetry in G1. inv G1.
+
+    st. unfold Fair. st.
+    iDestruct "GRT" as "%". iDestruct "GRT'" as "[W [_ %]]". subst.
+    force_l. 
+    instantiate (1:=middle_update isrc itgt y3).
+    st. force_l. iSplitR.
+    { iPureIntro. et. }
+
+    st. force_l. force_l. iSplitL "W"; iFrame; et. st. iSplit; et.
+
+    unfold IstFair. iPureIntro.
+    exists y, (middle_update isrc itgt y3).
+    esplits; et. ii. unfold middle_update in *.
+    des_ifs.
+    - specialize (H i). rewrite Heq0 in H. apply OrdArith.lt_from_nat. ss.
+    - specialize (H i). rewrite Heq0 in H. rewrite H.
+      specialize (H1 f i). repeat rewrite Heq in H1. ss.
+    - apply Ord.omega_upperbound.
+  Qed.
+
+  Theorem sim: 
+    forall (i_tgt: iimap id nat_wf),
+    HModPair.sim
+      (ModFairA.HFair i_omega)
+      (ModFairA.HFair i_tgt)
+      IstFair.
+  Proof.
+    ii. sim_init.
+    - rewrite// HFair_unfold. rewrite// HFair_unfold. s.
+      iIntros "E"; iFrame. unfold IstFair. iPureIntro. exists i_tgt. esplits; ss.
+      ii. unfold middle_update in *. des_ifs; ss. unfold i_omega. apply Ord.omega_upperbound.
+    - iApply simF_fair. ss.
+  Qed.
+
+
+  (* IST when target's imap only have a progress *)
+
+  Definition mirror_update isrc itgt f: iimap id owf := 
+    (fun x => match f x with
+              | Flag.success => (kappa)%ord
+              | Flag.fail => (Ord.omega + Ord.from_nat (itgt x))%ord
+              | _ => isrc x 
+              end).
+
+  Definition IstFairTgt: Any.t -> Any.t -> iProp :=
+    fun st_src st_tgt => 
+      (⌜exists (itgt: iimap id nat_wf) (isrc: iimap id owf), 
+        st_tgt = itgt↑ ∧ st_src = isrc↑
+        ∧ forall f, fair_update id owf isrc (mirror_update isrc itgt f) f⌝)%I.
+  
+  Definition i_kappa: iimap id owf := fun x => kappa.
+
+  Lemma simF_fair_tgt:
+    forall (i_tgt: iimap id nat_wf),
+    HModPair.sim_fun
+      (ModFairA.HFair i_kappa)
+      (ModFairA.HFair i_tgt)
+      IstFairTgt "fair".
+  Proof.
+    simF_init HFair_unfold HFair_unfold fairF fairF.
+    st. iDestruct "ASM" as "[W [% %]]"; des; subst.
+    
+    rewrite Any.upcast_downcast in G. inv G. ss. inv G0.
+
+    force_r. instantiate (1:=mk_meta y0 y1 ()). force_r. force_r. iSplitR "IST".
+    { iFrame; et. }
+    st. iDestruct "IST" as "%"; des; subst.
+    
+    rewrite Any.upcast_downcast in G1. symmetry in G1. inv G1.
+
+    st. unfold Fair. st.
+    iDestruct "GRT" as "%". iDestruct "GRT'" as "[W [_ %]]". subst.
+    force_l. 
+    instantiate (1:=mirror_update isrc itgt y3).
+    st. force_l. iSplitR.
+    { 
+      iPureIntro. unfold fair_update in *. i. specialize (H i). specialize (H1 y3 i). unfold mirror_update in *. des_ifs.
+    }
+
+    st. force_l. force_l. iSplitL "W"; iFrame; et. st. iSplit; et.
+
+    unfold IstFairTgt. iPureIntro. esplits; et.
+    ii. unfold fair_update, mirror_update in *. specialize (H i). des_ifs.
+    - apply OrdArith.lt_add_r. apply OrdArith.lt_from_nat. ss.
+    - ss. specialize (H1 f i). rewrite Heq in H1. rewrite H. ss.
+    - ss. apply kappa_inaccessible_add. apply kappa_inaccessible_omega. apply kappa_inaccessible_nat.
+  Qed.
+
+  Theorem sim_tgt: 
+    forall (i_tgt: iimap id nat_wf),
+    HModPair.sim
+      (ModFairA.HFair i_kappa)
+      (ModFairA.HFair i_tgt)
+      IstFairTgt.
+  Proof.
+    ii. sim_init.
+    - rewrite// HFair_unfold. rewrite// HFair_unfold. s.
+      iIntros "E"; iFrame. unfold IstFairTgt. iPureIntro. exists i_tgt. esplits; ss.
+      i. unfold fair_update, mirror_update. i. des_ifs.
+      apply kappa_inaccessible_add. apply kappa_inaccessible_omega. apply kappa_inaccessible_nat.
+    - iApply simF_fair_tgt. ss.
+  Qed.
+  
+End SIMMODSEM.
