examples/modfair/ModFairTestI.v
@@ -1,0 +1,64 @@
+Require Import Coqlib.
+Require Import ITreelib.
+Require Import ImpPrelude.
+Require Import STS.
+Require Import Behavior.
+Require Import ModSem.
+Require Import Skeleton.
+Require Import PCM.
+Require Import HoareDef STB IPM.
+
+Require Import sProp sWorld World SRF.
+From stdpp Require Import coPset gmap namespaces.
+
+Require Import FairCounter WFLibLarge ModFairA.
+
+Set Implicit Arguments.
+
+Section I.
+
+  Context `{_W: CtxWD.t}.
+
+  Definition ff (n: nat): Flag.t :=
+    if (n =? 0) then Flag.success else 
+      if (n =? 1) then Flag.fail else Flag.emp.
+
+  Definition testF: list val -> itree hAGEs val :=
+    fun varg =>
+      (* tau for progress *)
+      tau;; _ <- 
+      (ITree.iter
+        (fun (_: unit) =>
+          `b: bool <- trigger (Choose bool);;
+          if b
+          then
+            `_: val <- (ccallU "fair" [ff]);;
+            _ <- trigger (Syscall "print" [Vint 42]↑ top1);;
+            Ret (inl tt: unit + unit)
+          else 
+            `_: val <- (ccallU "fair" [ff]);;
+            Ret (inl tt: unit + unit)
+      ) tt);;
+      Ret Vundef
+  .
+
+  Definition FairSem: HModSem.t := {|
+    HModSem.fnsems := [("test", cfunU testF)];
+    HModSem.initial_st := tt↑;
+    HModSem.initial_cond := emp
+  |}
+  .
+
+  Definition _Fair: HMod.t := {|
+    HMod.get_modsem := fun _ => FairSem;
+    HMod.sk := [("test", Gfun↑)];
+  |}
+  .
+  Definition Fair := _Fair.
+  
+  Lemma Fair_unfold: Fair = _Fair.
+  Proof. eauto. Qed.
+
+  Global Opaque Fair.
+
+End I.
