examples/modfair/ModFairTestIAproof.v
@@ -1,0 +1,170 @@
+Require Import ModFairTestA ModFairTestI ModFairA ModFairAproof.
+Require Import HoareDef SimModSem.
+Require Import Coqlib.
+Require Import ImpPrelude.
+Require Import Skeleton.
+Require Import PCM.
+Require Import ModSem ModSemE Behavior.
+Require Import Relation_Definitions.
+
+(*** TODO: export these in Coqlib or Universe ***)
+Require Import Relation_Operators.
+Require Import RelationPairs.
+From ITree Require Import
+     Events.MapDefault.
+From ExtLib Require Import
+     Core.RelDec
+     Structures.Maps
+     Data.Map.FMapAList.
+Require Import HTactics ProofMode IPM.
+Require Import OpenDef.
+Require Import Mem1 STB Invariant.
+
+Require Import IProofMode IRed ITactics.
+
+Require Import sProp sWorld World SRF.
+From stdpp Require Import coPset gmap namespaces.
+
+Require Import WFLibLarge FairCounter.
+
+Set Implicit Arguments.
+
+Local Open Scope nat_scope.
+
+Section SIMMODSEM.
+  Context `{_W: CtxWD.t}.
+        
+  Variable GlobalStb: Sk.t -> gname -> option fspec.
+  Hypothesis STBINCLM: forall sk, stb_incl (to_stb (FairStb nat)) (GlobalStb sk).
+
+  Definition Ist: Any.t -> Any.t -> iProp :=
+    fun st_src st_tgt => (⌜True⌝)%I.
+
+  Ltac coapply :=
+    iApply isim_progress;
+    iApply isim_base;
+    match goal with [|- context[_ _ _ _ _ (?st_src, _) (?st_tgt, _)]] =>
+      iApply ("CIH" $! (@existT _ (λ _, _) st_src st_tgt)); eauto
+    end.
+
+  Definition i_kappa: iimap nat owf := @i_kappa nat.
+
+  Lemma simF_test:
+    forall i_tgt: iimap nat nat_wf,
+    HModPair.sim_fun
+      (HMod.add (ModFairTestA.HFair GlobalStb) (ModFairA.HFair i_kappa))
+      (HMod.add ModFairTestI.Fair (ModFairA.HFair i_tgt))
+      (IstProd Ist (IstFairTgt nat)) "test".
+  Proof.
+    simF_init ModFairTestA.HFair_unfold ModFairTestI.Fair_unfold ModFairTestA.testF ModFairTestI.testF.
+
+    st_l. hss. iDestruct "ASM" as "(W & (% & %Y))". subst. hss. st_r. grind.
+    iApply isim_progress.
+        
+    (* To prove a situation of infinity, use coinduction *)
+    iStopProof.
+    revert st_src st_tgt. apply combine_quant. (* boilerplate for coinduction *)
+    eapply isim_coind.
+    i. destruct a as [st_src st_tgt]. s.
+    iIntros "(#(_ & CIH) & [IST W])".
+    (* Now we can use a coinduction hypothesis *)
+    
+    rewrite// [X in isim _ _ _ _ _ _ _ _ (_, (translate _ (interp_hEs_hAGEs _ _ X)) >>= _) (_, _)] unfold_iter_eq.
+    rewrite// [X in isim _ _ _ _ _ _ _ _ (_, _) (_, (translate _ X) >>= _)] unfold_iter_eq.
+    st_r. destruct y.
+    
+    (* CASE 1: fair case *)
+    {
+      (* Inlining fair function *)
+      inline_r. s.
+      st_r. force_r. instantiate (1:=mk_meta y0 y1 ()). st_r. force_r. st_r. force_r.
+      iSplitR "IST".
+      { iFrame. iPureIntro. esplits; et. }
+      unfold ModFairA.fairF. st_r. unfold cfunU. hss.
+      iDestruct "IST" as (? ? ? ?) "[% [_ %]]". des; subst. 
+      st_r. hss. st_r. unfold Fair. st_r. hss. hss.
+      rename itgt into prev. rename y into next.
+      iDestruct "GRT" as "%". iDestruct "GRT'" as "[W [_ %]]"; des; subst. st_r.
+      st. coapply. iClear "CIH".
+      unfold IstProd, Ist, IstFairTgt. iFrame.
+      iExists (st_srcL), (st_tgtL), (isrc↑), (next↑). iSplit.
+      - iPureIntro. esplits; ss.
+      - iSplit; ss. iPureIntro. esplits; et. ii.
+        specialize (H2 f i). specialize (H i).
+        unfold fair_update, mirror_update in *. 
+        des_ifs; ss.
+        + admit.
+        + rewrite H. ss.
+        +
+        + etrans. apply OrdArith.lt_from_nat. eapply H. ss.
+        + rewrite H. ss.
+        + 
+    }
+    (* CASE 2: unfair case *)
+    {
+      inline_r. s.
+      st_r. force_r. instantiate (1:=mk_meta y0 y1 ()). st_r. force_r. st_r. force_r.
+      iSplitR "IST".
+      { iFrame. iPureIntro. esplits; et. }
+      unfold ModFairA.fairF. st_r. unfold cfunU. hss.
+      iDestruct "IST" as (? ? ? ?) "[% [_ %]]". des; subst.
+      st_r. hss. st_r. unfold Fair. st_r. hss. hss.
+      rename itgt into prev. rename y into next.
+      iDestruct "GRT" as "%". iDestruct "GRT'" as "[W [_ %]]"; des; subst. st_r.
+      unfold FairCounter.fair_update, ff in H. specialize (H 1). ss.
+
+      remember (prev 1) as chance. clear Heqchance. gen next.
+      induction chance.
+      { ii. inv H. }
+      {
+        ii. rewrite// [X in isim _ _ _ _ _ _ _ _ (_, _) (_, (translate _ X) >>= _)] unfold_iter_eq.
+        st_r. destruct y.
+        (* If the next case is fair, the previous unfair one won't be an issue. *)
+        {
+          st_r. inline_r. s. st_r. force_r. instantiate (1:=mk_meta y0 y1 ()). st_r. force_r.
+          st_r. force_r. iSplitL.
+          { iFrame. iPureIntro. et. }
+          unfold fairF. st_r. unfold cfunU. hss.
+          st_r. hss. st_r. unfold Fair. st_r. hss. hss.
+          iDestruct "GRT" as "%". iDestruct "GRT'" as "[W [_ %]]"; des; subst. st.
+          coapply. iClear "CIH".
+          unfold IstProd, Ist, IstFairTgt. iFrame.
+          iExists (st_srcL), (st_tgtL), (st_srcR), (y↑). iSplit; [|iSplit; esplits; et].
+          iPureIntro. esplits; ss.
+        }
+
+        (* Consecutive unfair case *)
+        {
+          st_r. inline_r. s. st_r. force_r. instantiate (1:=mk_meta y0 y1 ()). st_r. force_r. st_r.
+          force_r. iSplitL.
+          { iFrame; iPureIntro; et. }
+          unfold fairF. st_r. unfold cfunU. hss. st_r. hss. hss. st_r.
+          unfold Fair. st_r. hss. hss.
+          iDestruct "GRT" as "%". iDestruct "GRT'" as "[W [_ %]]"; des; subst. st_r.
+          apply IHchance. clear IHchance.
+          specialize (H0 1). ss. nia.
+        }
+      }
+    }
+  Qed.
+  
+  Theorem sim: 
+    forall ii, 
+      HModPair.sim 
+        (ModFairTestA.HFair GlobalStb)
+        (HMod.add ModFairTestI.Fair (ModFairA.HFair ii)) 
+        (IstProd Ist IstFairTgt).
+  Proof.
+    ii. 
+    econs; eauto; ii.
+    - Locate HModSemPair.sim.
+    econs. cycle 1; [s|sim_split].
+    sim_init.
+    - rewrite// ModFairTestA.HFair_unfold ModFairTestI.Fair_unfold. s.
+      iIntros "E"; iFrame. unfold IstProd. iExists _, _, _, _.
+      iSplit; ss. iSplit; ss. unfold IstFairTgt. iPureIntro. et.
+    - iApply simF_test. ss.
+    - 
+  Qed.
+  
+End SIMMODSEM.
